src/arch/x64/X64.Vale.Decls_i.fsti
@@ -139,13 +139,13 @@ let va_opr_lemma_Mem (s:va_state) (base:operand) (offset:int) (b:M.buffer64) (in
 
 (* Predicates *)
 [@va_qattr] unfold let va_is_src_opr64 (o:operand) (s:va_state) = valid_operand o s
-[@va_qattr] let va_is_dst_opr64 (o:operand) (s:va_state) = match o with OReg Rsp -> false | OReg _ -> true | _ -> false
+[@va_qattr] let va_is_dst_opr64 (o:operand) (s:va_state) = match o with OReg r -> r <> rsp | _ -> false
 [@va_qattr] unfold let va_is_dst_dst_opr64 (o:va_dst_operand) (s:va_state) = va_is_dst_opr64 o s
 [@va_qattr] unfold let va_is_src_reg (r:reg) (s:va_state) = True
 [@va_qattr] unfold let va_is_dst_reg (r:reg) (s:va_state) = True
 [@va_qattr] unfold let va_is_src_shift_amt64 (o:operand) (s:va_state) = valid_operand o s /\ (va_eval_shift_amt64 s o) < 64
 [@va_qattr] unfold let va_is_src_reg_opr64 (o:operand) (s:va_state) = OReg? o
-[@va_qattr] unfold let va_is_dst_reg_opr64 (o:operand) (s:va_state) = OReg? o /\ not (Rsp? (OReg?.r o))
+[@va_qattr] unfold let va_is_dst_reg_opr64 (o:operand) (s:va_state) = OReg? o /\ OReg?.r o <> rsp
 [@va_qattr] unfold let va_is_src_xmm (x:xmm) (s:va_state) = True
 [@va_qattr] unfold let va_is_dst_xmm (x:xmm) (s:va_state) = True
 
