src/arch/x64/X64.Vale.Regs_i.fsti
@@ -5,30 +5,10 @@ open X64.Machine_s
 
 type t = Map16_i.map nat64
 
-[@va_qattr]
-let reg_to_int (r:reg) : int =
-  match r with
-  | Rax -> 0
-  | Rbx -> 1
-  | Rcx -> 2
-  | Rdx -> 3
-  | Rsi -> 4
-  | Rdi -> 5
-  | Rbp -> 6
-  | Rsp -> 7
-  | R8 -> 8
-  | R9 -> 9
-  | R10 -> 10
-  | R11 -> 11
-  | R12 -> 12
-  | R13 -> 13
-  | R14 -> 14
-  | R15 -> 15
-
 val equal : regs1:t -> regs2:t -> Type0
 
 val lemma_equal_intro : regs1:t -> regs2:t -> Lemma
-  (requires forall r. Map16_i.sel regs1 (reg_to_int r) == Map16_i.sel regs2 (reg_to_int r))
+  (requires forall (r:reg). Map16_i.sel regs1 r == Map16_i.sel regs2 r)
   (ensures equal regs1 regs2)
   [SMTPat (equal regs1 regs2)]
 
