tools/Vale/test/StateUpdateTest.fst
@@ -8,28 +8,28 @@ open FStar.Tactics
 
 val va_code_state_update_test : va_dummy:unit -> Tot va_code
 let va_code_state_update_test () =
-  (va_Block (va_CCons (va_code_Mov64 (va_op_dst_operand_reg Rdx) (va_op_operand_reg Rax)) (va_CCons
-    (va_code_Mov64 (va_op_dst_operand_reg Rcx) (va_op_operand_reg Rdx)) (va_CNil ()))))
+  (va_Block (va_CCons (va_code_Mov64 (va_op_dst_operand_reg rdx) (va_op_operand_reg rax)) (va_CCons
+    (va_code_Mov64 (va_op_dst_operand_reg rcx) (va_op_operand_reg rdx)) (va_CNil ()))))
 
 irreducible val va_lemma_state_update_test : va_b0:va_codes -> va_s0:va_state -> va_sN:va_state
   -> Ghost ((va_bM:va_codes) * (va_sM:va_state))
   (requires ((va_require va_b0 (va_code_state_update_test ()) va_s0 va_sN) /\ (va_get_ok va_s0)))
   (ensures (fun ((va_bM:va_codes), (va_sM:va_state)) -> ((va_ensure va_b0 va_bM va_s0 va_sM va_sN)
-    /\ (va_get_ok va_sM) /\ (va_state_eq va_sM (va_update_reg Rcx va_sM (va_update_reg Rdx va_sM
+    /\ (va_get_ok va_sM) /\ (va_state_eq va_sM (va_update_reg rcx va_sM (va_update_reg rdx va_sM
     (va_update_ok va_sM va_s0)))))))
 irreducible let va_lemma_state_update_test va_b0 va_s0 va_sN =
   ();
   let (va_old_s:va_state) = va_s0 in
   let (va_sM, (va_cM:va_code), va_bM) = (va_lemma_block va_b0 va_s0 va_sN) in
   let (va_b1:va_codes) = (va_get_block va_cM) in
-  let (va_b2, va_s2) = (va_lemma_Mov64 va_b1 va_s0 va_sM (va_op_dst_operand_reg Rdx)
-    (va_op_operand_reg Rax)) in
+  let (va_b2, va_s2) = (va_lemma_Mov64 va_b1 va_s0 va_sM (va_op_dst_operand_reg rdx)
+    (va_op_operand_reg rax)) in
 
   // let upd_lemma (m : tmap int uint64) : Lemma
-  //   (ensures (m.[reg_to_int Rax] == 
-  // 			 (m.[reg_to_int Rdx] <- m.[reg_to_int Rax]).[reg_to_int Rax])) =
+  //   (ensures (m.[reg_to_int rax] == 
+  // 			 (m.[reg_to_int rdx] <- m.[reg_to_int rax]).[reg_to_int rax])) =
   //   assert_by_tactic (norm[Simpl;Delta;Primops];; dump "before trefl";; trivial;; dump "after trivial")
-  // 		   (m.[reg_to_int Rax] == (m.[reg_to_int Rdx] <- (m.[reg_to_int Rax])).[reg_to_int Rax])
+  // 		   (m.[reg_to_int rax] == (m.[reg_to_int rdx] <- (m.[reg_to_int rax])).[reg_to_int rax])
   // in
   //   upd_lemma (va_s0.regs);
 
@@ -38,18 +38,18 @@ irreducible let va_lemma_state_update_test va_b0 va_s0 va_sN =
         | (Mkstate _ __fname__regs#1094345 _ _)  -> __fname__regs@2) 0)*)
 
   // assert_by_tactic (norm[Simpl;Delta;Primops];; dump "before trivial";; trivial;; dump "trivial")
-  //   (va_s0.regs0.[reg_to_int Rax] == (va_s0.regs.[reg_to_int Rdx] <- va_s0.regs.[reg_to_int Rax]).[reg_to_int Rax]);
+  //   (va_s0.regs0.[reg_to_int rax] == (va_s0.regs.[reg_to_int rdx] <- va_s0.regs.[reg_to_int rax]).[reg_to_int rax]);
 
  (* We can destruct va_s0 without tactics *)
   let (Mkstate ok0 regs0 flags0 mem0 :va_state) = va_s0 in
   // and now this works.
-  let s1 = update_reg Rdx (regs0 Rax) (Mkstate ok0 regs0 flags0 mem0) in
-  assert_by_tactic (regs0 Rax == s1.regs Rax) (norm[simplify;delta;primops];; dump "before trefl";; trivial;; dump "trivial");
+  let s1 = update_reg rdx (regs0 rax) (Mkstate ok0 regs0 flags0 mem0) in
+  assert_by_tactic (regs0 rax == s1.regs rax) (norm[simplify;delta;primops];; dump "before trefl";; trivial;; dump "trivial");
 
-  let (va_b4, va_s4) = (va_lemma_Mov64 va_b2 va_s2 va_sM (va_op_dst_operand_reg Rcx)
-    (va_op_operand_reg Rdx)) in
+  let (va_b4, va_s4) = (va_lemma_Mov64 va_b2 va_s2 va_sM (va_op_dst_operand_reg rcx)
+    (va_op_operand_reg rdx)) in
 
-  assert ((va_get_reg Rax va_s4) == (va_get_reg Rax va_old_s));
+  assert ((va_get_reg rax va_s4) == (va_get_reg rax va_old_s));
   let va_sM = (va_lemma_empty va_s4 va_sM) in
   (va_bM, va_sM)
 *)
